\documentclass{article}
\usepackage{amsfonts}
\usepackage{amsmath}
\usepackage{hyperref}
\begin{document}
\section{Continuous}
	Solve
	\[
	-\nabla\sigma(u) = f,
	\]
	where $\sigma(x) = C:\varepsilon(u)$, 
		  $\varepsilon(u,x) = \frac{1}{2}(\nabla u + \nabla u^T)$.
	Auxiliary variable $\sigma = C\varepsilon(u)$.
	Multiply by test functions $v$ and $\tau$ and integrate by parts in each element $K$,
	\begin{align}
	\int_K \sigma \cdot \tau&=-\int_Ku\nabla\cdot \tau dx +\int_{\partial K}u \cdot n \tau ds\\
	\int_K \sigma \cdot \nabla v&=\int_K fv dx +\int_{\partial K}\sigma \cdot n v ds.
	\end{align}
	Substitute in numerical fluxes $\hat{u}$ and $\hat{\sigma}$ for boundary integrals.
	\begin{align}
	\int_K \sigma \cdot \tau&=-\int_Ku\nabla\cdot \tau dx +\int_{\partial K}\hat{u} n\cdot \tau ds \label{eq:aux}\\
	\int_K \sigma \cdot \nabla v&=\int_K fv dx +\int_{\partial K}\hat{\sigma} \cdot n v ds.
		\label{eq:force}
	\end{align}
	Integration by parts second time for $\int_Ku\nabla\cdot \tau dx$ in \autoref{eq:aux}:
	\begin{equation}
	\int_Ku\nabla\cdot \tau dx=\int_{\partial K}u n\cdot \tau-\int_K\nabla u\cdot \tau.
	\label{eq:ibp}
	\end{equation}
	Let $\tau=\nabla v$ and substitute \autoref{eq:ibp} into \autoref{eq:aux}:
	\begin{equation}
	\int_K \sigma \cdot \nabla v = -\int_{\partial K}u n\cdot \nabla v+\int_K\nabla u\cdot \nabla v +\int_{\partial K}\hat{u} n\cdot \nabla v ds 
	\label{eq:stress}
	\end{equation}
	Substitute \autoref{eq:stress} into \autoref{eq:force} to get
	\begin{equation}
	\int_K fvdx + \int_{\partial K}\hat{\sigma}\cdot nvds 
	= \int_{\partial K}(\hat{u}-u) n\cdot \nabla v+\int_K\nabla u\cdot \nabla v.
	\end{equation}
		
\section{Discrete}
	\[u(x)=\sum_{i=1}^{8}N_i(x)U_i = H(x)U\]
	\[U = \begin{pmatrix}
	u_{1,x} & u_{1,y} & u_{1,z} & u_{2,x} & u_{2,y} & u_{2,z} & ...\\
	\end{pmatrix}^T(24\times 1)\]
	\[H(x) = \begin{pmatrix}
	  N_1 & 0   & 0   & N_2 & 0   & 0   & ...\\
	  0   & N_1 & 0   & 0   & N_2 & 0   & ...\\
	  0   & 0   & N_1 & 0   & 0   & N_2 & ...\\	  	  
	\end{pmatrix}(3\times 24)\]
	\[B(x) = \begin{pmatrix}
	  \frac{\partial N_1}{\partial x_1} & 0 & 0& ...\\
	  0 & \frac{\partial N_1}{\partial x_2} & 0& ...\\
	  0 & 0 & \frac{\partial N_1}{\partial x_2}& ...\\
 	  \frac{\partial N_1}{\partial x_2} & \frac{\partial N_1}{\partial x_1} & 0& ...\\
  	  0 & \frac{\partial N_1}{\partial x_3} & \frac{\partial N_1}{\partial x_2}& ...\\
  	  \frac{\partial N_1}{\partial x_3} & 0 & \frac{\partial N_1}{\partial x_1}& ...
	\end{pmatrix}(6\times 24)\]
	\[\varepsilon(u,x) = B(x)U\]
	Choose $\hat{\sigma}=C\varepsilon(z)$, $\hat{u}=Z$.
	\[V\int_K B(x)CB(x)U + V\int_{\partial K}B^T(x)C^TN^TH(x)(Z-U)
	=V\int_K H^T(x)f+V\int_{\partial K}H(x)NCB(x)Z.\]
	Remove $V$.
	\[\int_K B(x)CB(x)U + \int_{\partial K}B^T(x)C^TN^TH(x)(Z-U)
	=\int_K H^T(x)f + \int_{\partial K}H(x)NCB(x)Z.\]
	
	\[
	N = \begin{pmatrix}
	n_x & 0   & 0   & n_y & 0   & n_z\\
	0   & n_y & 0   & n_x & n_z & 0 \\
	0   & 0   & n_z & 0   & n_y & n_x  \\		
	\end{pmatrix}(3\times 6)
	\]
	In reference space
	\[KU + \int_{\partial K}P(x)N^TH(x)(Z-U)
	=\int_K H^T(x)f + \int_{\partial K}H(x)NP(x)Z.\]
	Let $T=\int_{\partial K}H(x)NP(x)$, $F = \int_K H^T(x)f$, rearrange
	\[(K-T^T)U=F + (T-T^T)Z.\]
	
\section{Linear Material}
	P(x) = E(x)B(x)
\end{document}